standard_typing/coq/typing.v
@@ -1,0 +1,723 @@
+
+(*
+This file is created on April 22, 2021
+
+syntax.v is the syntax file for this semantics
+
+April 22, 2020:
+---------------
+-> Bidirectional to standard typing judgement
+
+*)
+
+Require Import TLC.LibLN.
+Require Import syntax.
+
+(** definitions *)
+
+(* defns value *)
+Inductive value : exp -> Prop :=    (* defn value *)
+ | val_int : forall i5,
+     value (e_lit i5)
+ | val_abs : forall e,
+     lc_exp (e_abs e) ->
+     value (e_abs e).
+
+(* defns FindType *)
+Inductive findtype : exp -> typ -> Prop :=    (* defn findtype *)
+ | findtype_int : forall i5,
+     findtype (e_lit i5) t_int
+ | findtype_arrow : forall (e:exp),
+     lc_exp (e_abs e) ->
+     findtype  (e_abs e) (t_arrow t_top t_bot).
+
+Hint Constructors value findtype : core.
+
+(* defns Typing *)
+Inductive typing : env -> exp -> typ -> Prop :=    (* defn typing *)
+ | typ_lit : forall (G:env) i5,
+      okt  G  ->
+     typing G (e_lit i5) t_int
+ | typ_var : forall (G:env) (x:var) (A:typ),
+      okt  G  ->
+      binds  x A G  ->
+     typing G (e_var_f x) A
+ | typ_app : forall (G:env) (e1 e2:exp) (B A:typ),
+     typing G e1 (t_arrow A B) ->
+     typing G e2 A ->
+     typing G (e_app e1 e2) B
+ | typ_sub : forall (G:env) (e:exp) (A B:typ),
+     typing G e B ->
+     B <: A ->
+     typing G e A
+ | typ_abs : forall (L:vars) (G:env) (e:exp) (A B:typ),
+      ( forall x , x \notin  L  -> typing  (G & x ~: A )   ( open_exp_wrt_exp e (e_var_f x) ) B )  ->
+     typing G (e_abs e) (t_arrow A B)
+ | typ_typeof : forall (L:vars) (G:env) (e:exp) (A:typ) (e1:exp) (B:typ) (e2:exp) (C:typ),
+     typing G e (t_union A B) ->
+     ( forall x , x \notin  L  -> typing  (G & x ~: A )   ( open_exp_wrt_exp e1 (e_var_f x) ) C ) ->
+     ( forall x , x \notin  L  -> typing  (G & x ~: B )   ( open_exp_wrt_exp e2 (e_var_f x) ) C ) ->
+     A *s B ->
+     typing G (e_typeof e A e1 B e2) C.
+
+(* defns Reduction *)
+Reserved Notation "e --> e'" (at level 80).
+Inductive step : exp -> exp -> Prop :=    (* defn step *)
+ | step_appl : forall (e1 e2 e1':exp),
+     lc_exp e2 ->
+     e1 --> e1' ->
+     (e_app e1 e2) --> (e_app e1' e2)
+ | step_appr : forall (v e e':exp),
+     value v ->
+     e --> e' ->
+     (e_app v e) --> (e_app v e')
+ | step_beta : forall (e:exp) (v:exp),
+     lc_exp (e_abs e) ->
+     value v ->
+     e_app  (e_abs e) v --> (open_exp_wrt_exp e v)
+ | step_typeof : forall (e:exp) (A:typ) (e1:exp) (B:typ) (e2 e':exp),
+     lc_exp (e_typeof e A e1 B e2) ->
+     e --> e' ->
+     (e_typeof e A e1 B e2) --> (e_typeof e' A e1 B e2)
+ | step_typeofl : forall (v:exp) (A:typ) (e1:exp) (B:typ) (e2:exp) (C:typ),
+     lc_exp (e_typeof v A e1 B e2) ->
+     value v ->
+     findtype v C ->
+     C <: A ->
+     (e_typeof v A e1 B e2) -->  (open_exp_wrt_exp e1 v)
+ | step_typeofr : forall (v:exp) (A:typ) (e1:exp) (B:typ) (e2:exp) (C:typ),
+    lc_exp (e_typeof v A e1 B e2) ->
+     value v ->
+     findtype v C ->
+     C <: B ->
+     (e_typeof v A e1 B e2) -->  (open_exp_wrt_exp  e2 v )
+where "e --> e'" := (step e e') : env_scope.
+
+Hint Constructors typing step : core.
+
+
+(** Gathering free names already used in the proofs *)
+
+
+Ltac gather_vars :=
+  let A := gather_vars_with (fun x : vars => x) in
+  let B := gather_vars_with (fun x : var => \{x}) in
+  let D := gather_vars_with (fun x : exp => fv_exp x) in
+  let F := gather_vars_with (fun x : env => dom x) in
+  constr:(A \u B \u D \u F).
+
+(** "pick_fresh x" tactic create a fresh variable with name x *)
+
+Ltac pick_fresh x :=
+  let L := gather_vars in (pick_fresh_gen L x).
+
+(** "apply_fresh T as x" is used to apply inductive rule which
+   use an universal quantification over a cofinite set *)
+
+Tactic Notation "apply_fresh" constr(T) "as" ident(x) :=
+  apply_fresh_base T gather_vars x.
+
+Tactic Notation "apply_fresh" "*" constr(T) "as" ident(x) :=
+  apply_fresh T as x; autos*.
+
+(** These tactics help applying a lemma which conclusion mentions
+  an environment (E & F) in the particular case when F is empty *)
+
+Ltac get_env :=
+  match goal with
+  | |- subtyping ?E _ _  => E
+  | |- typing ?E _ _ => E
+  end.
+
+Tactic Notation "apply_empty_bis" tactic(get_env) constr(lemma) :=
+  let E := get_env in rewrite <- (concat_empty_r E);
+  eapply lemma; try rewrite concat_empty_r.
+
+Tactic Notation "apply_empty" constr(F) :=
+  apply_empty_bis (get_env) F.
+
+Tactic Notation "apply_empty" "*" constr(F) :=
+  apply_empty F; autos*.
+
+
+(* ********************************************************************** *)
+(** ** Properties of term substitution in terms *)
+
+Lemma open_ee_rec_term_core : forall e j v u i, i <> j ->
+open_exp_wrt_exp_rec j v e = open_exp_wrt_exp_rec i u (open_exp_wrt_exp_rec j v e) ->
+  e = open_exp_wrt_exp_rec i u e.
+Proof.
+  induction e; introv Neq H; simpl in *; inversion H; f_equal*.
+  case_nat*. case_nat*.
+Qed.
+
+Lemma open_ee_rec_term : forall u e,
+  lc_exp e -> forall k, e = open_exp_wrt_exp_rec k u e.
+Proof.
+  induction 1; intros; simpl; f_equal*.
+  unfolds open_exp_wrt_exp. pick_fresh x.
+   apply* (@open_ee_rec_term_core e 0 (e_var_f x)).
+  unfolds open_exp_wrt_exp. pick_fresh x.
+   apply* (@open_ee_rec_term_core e1 0 (e_var_f x)).
+  unfolds open_exp_wrt_exp. pick_fresh x.
+   apply* (@open_ee_rec_term_core e2 0 (e_var_f x)).
+Qed.
+
+(** Substitution for a fresh name is identity. *)
+
+Lemma subst_ee_fresh : forall x u e,
+  x \notin fv_exp e -> subst_exp u x e = e.
+Proof.
+  induction e; simpl; intros; f_equal*.
+  case_var*.
+Qed.
+
+(** Substitution distributes on the open operation. *)
+
+Lemma subst_ee_open_ee : forall t1 t2 u x, lc_exp u ->
+subst_exp u x (open_exp_wrt_exp t1 t2) =
+open_exp_wrt_exp (subst_exp u x t1) (subst_exp u x t2).
+Proof.
+  intros. unfold open_exp_wrt_exp. generalize 0.
+  induction t1; intros; simpls; f_equal*.
+  case_nat*.
+  case_var*. rewrite* <- open_ee_rec_term.
+Qed.
+
+(** Substitution and open_var for distinct names commute. *)
+
+Lemma subst_ee_open_ee_var : forall x y u e, y <> x -> lc_exp u ->
+  (subst_exp u x e) open_ee_var y = subst_exp u x (e open_ee_var y).
+Proof.
+  introv Neq Wu. rewrite* subst_ee_open_ee.
+  simpl. case_var*.
+Qed.
+
+(** Opening up a body t with a type u is the same as opening
+  up the abstraction with a fresh name x and then substituting u for x. *)
+
+Lemma subst_ee_intro : forall x u e,
+  x \notin fv_exp e -> lc_exp u ->
+  open_exp_wrt_exp e u = subst_exp u x (e open_ee_var x).
+Proof.
+  introv Fr Wu. rewrite* subst_ee_open_ee.
+  rewrite* subst_ee_fresh. simpl. case_var*.
+Qed.
+
+(** Substitutions preserve local closure. *)
+
+Lemma subst_ee_term : forall e1 Z e2,
+lc_exp e1 -> lc_exp e2 -> lc_exp (subst_exp e2 Z e1).
+Proof.
+  induction 1; intros; simpl; auto.
+  case_var*.
+ - apply_fresh* lc_e_abs as y.
+   rewrite* subst_ee_open_ee_var.
+ - apply_fresh* lc_e_typeof as y.
+   rewrite* subst_ee_open_ee_var.
+   rewrite* subst_ee_open_ee_var.
+Qed.
+
+Hint Resolve subst_ee_term : core.
+
+(* ********************************************************************** *)
+(** * Relations between well-formed environment and types well-formed
+  in environments *)
+
+(** If an environment is well-formed, then it does not contain duplicated keys. *)
+
+Lemma ok_from_okt : forall E,
+  okt E -> ok E.
+Proof.
+  induction 1; auto.
+Qed.
+
+Hint Extern 1 (ok _) => apply ok_from_okt : core.
+
+
+(* ********************************************************************** *)
+(** ** Properties of well-formedness of an environment *)
+
+(** Inversion lemma *)
+
+Lemma okt_push_inv : forall E x T,
+  okt (E & x ~: T) -> okt E /\ x # E.
+Proof.
+  introv O. inverts O.
+    false* empty_push_inv.
+    lets (?&M&?): (eq_push_inv H). subst. autos.
+Qed.
+
+(** Through strengthening *)
+
+Lemma okt_strengthen : forall x T (E F:env),
+  okt (E & x ~: T & F) ->
+  okt (E & F).
+Proof.
+  introv O. induction F using env_ind.
+  rewrite concat_empty_r in *. apply okt_push_inv in O. destruct~ O.
+  rewrite concat_assoc in *.
+  apply okt_push_inv in O.
+  destruct O. apply IHF in H.
+  apply okt_typ; autos*.
+Qed.
+
+(** Automation *)
+
+Hint Immediate okt_strengthen : core.
+
+(* ********************************************************************** *)
+(** ** Regularity of relations *)
+
+(** The subtyping relation is restricted to well-formed objects. *)
+
+(** The typing relation is restricted to well-formed objects. *)
+
+Lemma typing_regular : forall E e T,
+  typing E e T -> okt E /\ lc_exp e.
+Proof.
+  induction 1; try splits*.
+ - pick_fresh y. specializes H0 y. destructs~ H0.
+  apply okt_push_inv in H0. destruct H0. auto.
+ - apply lc_e_abs with (L:=L). intros.
+  specializes H0 x. destructs~ H0.
+ - apply lc_e_typeof with (L:=L); intros. destruct~ IHtyping.
+   specialize (H1 x H5). destruct~ H1.
+   specialize (H3 x H5). destruct~ H3.
+Qed.
+
+(** The value relation is restricted to well-formed objects. *)
+
+Lemma value_regular : forall t,
+  value t -> lc_exp t.
+Proof.
+  induction 1; autos*.
+Qed.
+
+Hint Immediate value_regular : core.
+
+(* ********************************************************************** *)
+(** Weakening (5) *)
+
+
+Lemma typing_weakening : forall E F G e T,
+   typing (E & G) e T ->
+   okt (E & F & G) ->
+   typing (E & F & G) e T.
+Proof.
+  introv Typ. gen F. inductions Typ; introv Ok.
+  - apply* typ_lit.
+  - apply* typ_var. apply* binds_weaken.
+  - apply* typ_app.
+  - apply* typ_sub.
+  - apply_fresh* typ_abs as x.
+    forwards~: (H x).
+    apply_ih_bind (H0 x); eauto.
+  - apply_fresh* typ_typeof as x.
+    forwards*: H x. apply_ih_bind (H0 x); eauto.
+    forwards*: H1 x. apply_ih_bind (H2 x); eauto.
+Qed.
+
+(************************************************************************ *)
+(** Preservation by Term Substitution (8) *)
+
+Require Import Program.Equality.
+
+Lemma typing_through_subst_ee : forall E F x T e u U,
+   typing (E & x ~: U & F) e T ->
+   typing E u U ->
+   typing (E & F) (subst_exp u x e) T.
+Proof.
+introv TypT TypU.
+lets TypT': TypT.
+inductions TypT; introv; simpl.
+(*case int*)
+ - apply* typ_lit.
+(*case var*)
+ - case_var.
+  + binds_get H0.
+    lets M: (typing_weakening E F empty u U).
+    do 2 rewrite concat_empty_r in M.
+    apply* M.
+  + binds_cases H0; apply* typ_var.
+(*case app*)
+ - eapply typ_app; eauto.
+(*case sub*)
+ - eapply typ_sub; eauto.
+(*case abs*)
+ - apply_fresh* typ_abs as y.
+   assert (y \notin L) by auto.
+   specialize (H y H1).
+   rewrite* subst_ee_open_ee_var.
+   lets : H0 y H1 E (F & y ~: A) x.
+   lets : H2 U.
+   forwards* : H3.
+   rewrite~ concat_assoc.
+   rewrite~ concat_assoc.
+   rewrite~ <- concat_assoc.
+   apply typing_regular in TypU. destruct~ TypU.
+(*case typeof*)
+ - apply_fresh* typ_typeof as y.
+ + assert (y \notin L) by auto.
+   rewrite* subst_ee_open_ee_var.
+   lets: H y H4.
+   lets: H0 y H4 E (F & y ~: A) x.
+   lets: H6 U.
+   forwards*: H7.
+   rewrite~ concat_assoc.
+   rewrite~ concat_assoc.
+   rewrite~ <- concat_assoc.
+   apply typing_regular in TypU. destruct~ TypU.
++ assert (y \notin L) by auto.
+   rewrite* subst_ee_open_ee_var.
+   lets: H1 y H4.
+   lets: H2 y H4 E (F & y ~: B) x.
+   lets: H6 U.
+   forwards*: H7.
+   rewrite~ concat_assoc.
+   rewrite~ concat_assoc.
+   rewrite~ <- concat_assoc.
+   apply typing_regular in TypU. destruct~ TypU.
+Qed.
+
+
+(* ********************************************************************** *)
+(** Preservation Result (20) *)
+
+Lemma inv_int : forall E A i5,
+typing E (e_lit i5) A -> typing E (e_lit i5) t_int /\ t_int <: A.
+Proof.
+  introv Typ.
+  inductions Typ. 
+  (*case typ_int*)
+ - split*.
+  (*case typ_sub*)
+ - specialize (IHTyp i5).
+  forwards*: IHTyp. destruct H0.
+  split*.
+  eapply sub_transitivity; eauto.
+Qed.
+
+Lemma inv_arrow : forall G e A, 
+typing G (e_abs e) A ->
+exists A1 B1, (exists L, forall x , x \notin  L ->
+typing (G & x ~: A1) (e open_ee_var x) B1) /\ (t_arrow A1 B1) <: A.
+Proof.
+  introv Typ.
+  inductions Typ.
+  forwards*: IHTyp.
+  destruct H0 as [y [z]].
+  exists y z . destruct H0.
+  split*.
+  eapply sub_transitivity; eauto.
+  exists A B.
+  split*.
+Qed.
+
+Lemma check_or_typ : forall E e A B,
+   value e ->
+   typing E e (t_union A B) ->
+   typing E e A \/ typing E e B.
+Proof.
+  intros.
+  inverts H.
+  (*subsumption again*)
+ - apply inv_int in H0. destruct H0.
+   inverts* H0.
+ - apply inv_arrow in H0.
+   destruct H0 as [A1 [B1]].
+   destruct H as [H].
+   destruct H as [L].
+   inverts* H0.
+Qed.
+
+Lemma val_check_disjoint_types : forall E v A B,
+A *s B ->
+value v ->
+typing E v A ->
+typing E v B -> False.
+Proof.
+  introv Disj Val Typ1 Typ2.
+  unfold DisjSpec in Disj. unfold not in Disj.
+  inverts Val.
+  apply inv_int in Typ1. destruct Typ1.
+  apply inv_int in Typ2. destruct Typ2.
+  forwards*: Disj t_int.
+  apply inv_arrow in Typ1.
+  destruct Typ1 as [A1 [B1]]. destruct H0.
+  assert ((t_arrow t_top t_bot) <: (t_arrow A1 B1)). auto.
+  apply inv_arrow in Typ2.
+  destruct Typ2 as [A2 [B2]]. destruct H3.
+  assert ((t_arrow t_top t_bot) <: (t_arrow A2 B2)). auto.
+  eapply sub_transitivity with (A:=(t_arrow t_top t_bot)) (B:=(t_arrow A1 B1)) (C:=A) in H2; auto.
+  eapply sub_transitivity with (A:=(t_arrow t_top t_bot)) (B:=(t_arrow A2 B2)) (C:=B) in H5; auto.
+  forwards*: Disj (t_arrow t_top t_bot).
+Qed.
+
+Lemma check_find_type : forall E e A B,
+typing E e A ->
+findtype e B ->
+B <: A.
+Proof.
+  introv Typ Find.
+  inductions Find.
+  apply inv_int in Typ.
+  destruct~ Typ.
+  apply inv_arrow in Typ.
+  destruct Typ as [A1 [B1]].
+  destruct H0. destruct H0 as [L].
+  assert ((t_arrow t_top t_bot) <: (t_arrow A1 B1)) by auto.
+  eapply sub_transitivity; eauto.
+Qed.
+
+(*******************************)
+(****  Preservation Lemma  *****)
+(*******************************)
+
+Lemma preservation : forall E e e' T,
+  typing E e T ->
+  e --> e' ->
+  typing E e' T.
+Proof.
+  introv Typ. gen e'.
+  induction Typ; introv Red; try solve [ inverts* Red ].
+  - (* app *)
+    inverts* Red.
+    (* beta *)
+        forwards [A1 [B1]]: inv_arrow Typ1.
+        destruct H.
+        destruct H as [L].
+        inverts H0.
+        pick_fresh x.
+        assert (x \notin L) by auto.
+        lets: H x H0.
+        assert (G & x ~: A1 = G & x ~: A1 & empty).
+        rewrite* concat_empty_r.
+        rewrite H4 in H2.
+        assert (G = G & empty).
+        rewrite* concat_empty_r. rewrite H5.
+        lets: typing_through_subst_ee.
+        forwards*: H7 H2.
+        rewrite* (@subst_ee_intro x).
+        inverts H2.
+  - (* typeof *)
+    inverts* Red.
+    + (* value checks against disjoint types *)
+      lets temp: check_or_typ G e A B H11.
+      lets DisjOr: temp Typ.
+      destruct DisjOr.
+     * (*true goal*)
+       pick_fresh y. assert (y \notin L) by auto.
+       forwards*: H H5.
+       assert  (G & y ~: A = G & y ~: A & empty).
+       rewrite* concat_empty_r. rewrite H7 in H6.
+       assert (G = G & empty).
+       rewrite* concat_empty_r.
+       rewrite H8.
+       forwards*: typing_through_subst_ee.
+       rewrite* (@subst_ee_intro y).
+     * (*false goal, value e checks against disjoint types A and B*)
+       lets temp1: check_find_type G e B C0 H4.
+       lets SubB: temp1 H12.
+       unfold DisjSpec in H3. unfold not in H3.
+       destruct H12.
+       forwards*: H3 t_int.
+       forwards*: H3 (t_arrow t_top t_bot).
+    +  (* value checks against disjoint types *)
+      lets temp: check_or_typ G e A B H11.
+      lets DisjOr: temp Typ.
+      destruct DisjOr.
+     * (*false goal, value e checks against disjoint types A and B*)
+        lets temp1: check_find_type G e A C0 H4.
+        lets SubA: temp1 H12.
+        unfold DisjSpec in H3. unfold not in H3.
+        destruct H12.
+        forwards*: H3 t_int.
+        forwards*: H3 (t_arrow t_top t_bot).
+     * (*true goal*)  
+        pick_fresh y. assert (y \notin L) by auto.
+        forwards*: H1 H5.
+        assert  (G & y ~: B = G & y ~: B & empty).
+        rewrite* concat_empty_r. rewrite H7 in H6.
+        assert (G = G & empty).
+        rewrite* concat_empty_r.
+        rewrite H8.
+        forwards*: typing_through_subst_ee.
+        rewrite* (@subst_ee_intro y).
+Qed.
+
+
+(*******************************)
+(******  Progress Lemma  *******)
+(*******************************)
+
+Lemma progress : forall e T,
+typing empty e T -> (value e) \/ (exists e', e --> e').
+Proof.
+introv Typ. gen_eq E: (@empty typ). lets Typ': Typ.
+inductions Typ; intros EQ; subst.
+(*case int*)
+ - left*.
+ (*case var*)
+ - apply binds_empty_inv in H0. inversion H0.
+ (*case typ-app*)
+ - right. destruct* IHTyp1.
+  + destruct* IHTyp2.
+   * inverts* H.
+     (*i infers arrow*)
+     apply inv_int in Typ1.
+     destruct Typ1.
+     inverts H1. inverts H2.
+     (*case step-appl*)
+   * destruct H0.
+     exists* (e_app e1 x).
+   (*case step-appr*)
+  + destruct H. 
+    exists (e_app x e2). apply* step_appl.
+    forwards*: typing_regular Typ2.
+(*case typ-sub*)
+ - destruct~ IHTyp.
+(*case typ-abs*)
+ - left. forwards*: typing_regular Typ'.
+(*case typ-typeof*)
+ - right. destruct* IHTyp.
+  + apply check_or_typ in Typ; auto.
+    destruct Typ.
+    (*case typeofl*)
+   * destruct H4.
+     apply inv_int in H5. destruct H5.
+     { (*case e = int*)
+      exists (open_exp_wrt_exp e1 (e_lit i5)).
+      pick_fresh y.
+      assert (y \notin L) by auto.
+      lets: H y H6.
+      eapply step_typeofl with (C:=t_int); eauto.
+      forwards*: typing_regular Typ'.
+     }
+     { (*case e = \x.e*)
+      apply inv_arrow in H5.
+      destruct H5 as [A1 [B1]]. destruct H5.
+      assert ((t_arrow t_top t_bot) <: (t_arrow A1 B1)) by auto.
+      eapply sub_transitivity in H6; eauto.
+      exists (open_exp_wrt_exp e1 (e_abs e)).
+      pick_fresh y.
+      assert (y \notin L) by auto.
+      lets: H y H8.
+      eapply step_typeofl with (C:=(t_arrow t_top t_bot)); eauto.
+      forwards*: typing_regular Typ'.
+     }
+   * (*case typeofr*)
+     destruct H4.
+     apply inv_int in H5. destruct H5.
+     { (*case e = int*) 
+      exists (open_exp_wrt_exp e2 (e_lit i5)).
+      pick_fresh y.
+      assert (y \notin L) by auto.
+      lets: H1 y H6.
+      eapply step_typeofr with (C:=t_int); eauto.
+      forwards*: typing_regular Typ'.
+     }
+     { (*case e = \x.e*)
+      apply inv_arrow in H5.
+      destruct H5 as [A1 [B1]]. destruct H5.
+      assert ((t_arrow t_top t_bot) <: (t_arrow A1 B1)) by auto.
+      eapply sub_transitivity in H6; eauto.
+      exists (open_exp_wrt_exp e2 (e_abs e)).
+      pick_fresh y.
+      assert (y \notin L) by auto.
+      lets: H1 y H8.
+      eapply step_typeofr with (C:=(t_arrow t_top t_bot)); eauto.
+      forwards*: typing_regular Typ'.
+     }
+  + (*case typeof*)
+    destruct H4.
+    exists (e_typeof x A e1 B e2).
+    apply step_typeof; auto.
+    forwards*: typing_regular Typ'.
+Qed.
+
+(*******************************)
+(*****  Determinism Lemma  *****)
+(*******************************)
+
+Lemma inv_app : forall E e1 e2 A,
+typing E (e_app e1 e2) A ->
+exists A1 B1, typing E e1 (t_arrow A1 B1) /\ typing E e2 A1.
+Proof.
+  introv Typ.
+  inductions Typ.
+  exists* A B.
+  specialize (IHTyp e1 e2).
+  forwards*: IHTyp.
+Qed.
+
+Lemma inv_typeof : forall E e e1 e2 A B C,
+typing E (e_typeof e A e1 B e2) C ->
+exists D, typing E e D /\ A *s B.
+Proof.
+  introv Typ.
+  inductions Typ.
+  specialize (IHTyp e e1 e2 A B).
+  forwards*: IHTyp.
+  exists* (t_union A B).
+Qed.
+
+Lemma determinism_dir : forall E e e1 e2 A, typing E e A -> 
+e --> e1 -> e --> e2 -> e1 = e2.
+Proof.
+  introv Typ He1. gen e2 A.
+  induction He1; introv Typ He2.
+  (*case step-appl*)
+  - inverts* He2.
+   + apply inv_app in Typ.
+     destruct Typ as [A1 [B1]]. destruct H0.
+     forwards*: IHHe1. rewrite* H3.
+   + inverts* H2; inverts He1.
+   + inverts* He1.
+(*case step-appr*)
+  - inverts* He2.
+   + inverts* H; inverts* H4.
+   + apply inv_app in Typ.
+     destruct Typ as [A1 [B1]]. destruct H0.
+     forwards*: IHHe1 H1. rewrite* H3.
+   + inverts H4; inverts He1.
+(*case step-beta*)
+  - inverts* He2.
+   + inverts* H5. 
+   + inverts H0; inverts H5.
+(*case step-typeof*)
+ - inverts* He2.
+  + apply inv_typeof in Typ.
+    destruct Typ as [D]. destruct H0.
+    forwards*: IHHe1. rewrite* H2.
+  + inverts H8; inverts He1.
+  + inverts H8; inverts He1.
+(*case step-typeofl*)
+ - inverts* He2.
+  + inverts H0. inverts H10. inverts H10.
+  + apply inv_typeof in Typ.
+    destruct Typ as [D]. destruct H3 as [H3 Disj].
+    inverts H0.
+    * inverts H1.
+      inverts H11.
+      unfold DisjSpec in Disj. unfold not in Disj.
+      forwards*: Disj t_int.
+    * inverts H1.
+      inverts H11.
+      unfold DisjSpec in Disj. unfold not in Disj.
+      forwards*: Disj (t_arrow t_top t_bot).
+(*case step-typeofr*) 
+- inverts* He2.
+  + inverts H0; inverts H10. 
+  + apply inv_typeof in Typ.
+    destruct Typ as [D]. destruct H3 as [H3 Disj].
+    inverts H0.
+    * inverts H1.
+      inverts H11.
+      unfold DisjSpec in Disj. unfold not in Disj.
+      forwards*: Disj t_int.
+    * inverts H1.
+      inverts H11.
+      unfold DisjSpec in Disj. unfold not in Disj.
+      forwards*: Disj (t_arrow t_top t_bot).
+Qed.
